src/PlutusIR.v
@@ -286,21 +286,7 @@ Section ty__ind.
     (H_Builtin : forall (T : DefaultUni), P (Ty_Builtin T))
     (H_Lam : forall (X : binderTyname) (K : kind) (T : ty), P T -> P (Ty_Lam X K T))
     (H_App : forall (T1 T2 : ty), P T1 -> P T2 -> P (Ty_App T1 T2))
-    (H_SOP : forall (Tss : list (list ty)), ForallP22 P Tss -> P (Ty_SOP Tss)).
-
-  Definition tyss__ind (tys_rect : forall (ts : list ty), ForallP P ts) (ty_rect : forall (t : ty), P t) :=
-    fix tyss_rect' (tss : list (list ty)) :=
-    match tss as p return ForallP22 P p with
-      | nil       => ForallP2_nil P
-      | cons ts tss => ForallP2_cons P (tys_rect ts) (tyss_rect' tss)
-    end.
-
-  Definition tys__ind (ty_rect : forall (t : ty), P t) :=
-    fix tys_rect (ts : list ty) : ForallP P ts :=
-    match ts as p return ForallP P p with
-      | nil       => ForallP_nil
-      | cons t ts => ForallP_cons (ty_rect t) (tys_rect ts)
-    end.
+    (H_SOP : forall (Tss : list (list ty)), Forall (Forall P) Tss -> P (Ty_SOP Tss)).
 
   (* Main induction principle for `ty` *)
   Fixpoint ty__ind (T : ty) : P T :=
@@ -312,7 +298,20 @@ Section ty__ind.
     | Ty_Builtin T => H_Builtin T
     | Ty_Lam X K T => H_Lam X K T (ty__ind T)
     | Ty_App T1 T2 => H_App T1 T2 (ty__ind T1) (ty__ind T2)
-    | Ty_SOP Tss => H_SOP Tss (tyss__ind (tys__ind ty__ind) ty__ind Tss)
+    | Ty_SOP Tss =>
+        H_SOP Tss ((fix list_list_ind (tss : list (list ty)) : Forall (Forall P) tss :=
+          match tss with
+          | nil => Forall_nil _
+          | ts :: tss' =>
+              Forall_cons _
+                ((fix list_ind (ts : list ty) : Forall P ts :=
+                   match ts with
+                   | nil => Forall_nil _
+                   | t :: ts' => 
+                       Forall_cons _ (ty__ind t) (list_ind ts')
+                   end) ts)
+                (list_list_ind tss')
+          end) Tss)
     end.
 
 End ty__ind.
